Sodium.lean
@@ -1,8 +1,24 @@
 import «Sodium».Typo.Frontend.Qwerty
 
+open Lean Elab Tactic PrettyPrinter Sodium Crypto Ethos Typo Aesop
+
 universe «u»
 
-open Lean Sodium Crypto Ethos
+variable {τ : Sodium Universal.Destruct.{«u»}}
+
+attribute [aesop norm 0] Universal.universal_idx Universal.universal_default_idx
+
+attribute [aesop safe cases (rule_sets := [«external»])]
+  WType
+
+attribute [aesop safe forward (rule_sets := [«external»])]
+  PFunctor.W.head
+
+attribute [aesop norm 2 unfold (rule_sets := [«external»])]
+  PFunctor.W.children
+
+attribute [aesop safe apply (rule_sets := [«external»])]
+  PFunctor.W.cases
 
 /--
 HACK: This is a workaround for ensuring that `aesop`'s proof reconstruction works.
@@ -15,11 +31,68 @@ def construct : @default Prop prompt := by
   unfold prompt Universal.prompt
   simp only [Encodable.encodek, implies_true, and_self]
 
-@[aesop unsafe 0% apply (rule_sets := [«external»])] -- 0% to force termination before any "impossible" tactics are run.
+@[aesop unsafe apply (rule_sets := [«external»])]
 def destruct (fwd : Universal.Forward.{«u»}) : Universal Universal.Destruct.{«u»} := by
   refine ⟨default, fun α => ?_⟩
   have : Observable := α construct
   exact ⟨fwd this.carrier⟩
 
-example : Universal Universal.Destruct.{0} := by
-  aesop? (rule_sets := [«standard», «cautious», «external»])
+def framerule : RuleTac := RuleTac.ofTacticSyntax fun δ => do
+  match ← δ.goal.getType with
+  | .forallE _ (.app (.const ``Sodium [levelZero]) (.const ``Universal.Destruct [levelOne])) body _ =>
+    unless ← Meta.isLevelDefEq levelZero levelOne do Meta.throwIsDefEqStuck
+    CryptoM.toMetaM fun τ : Sodium Universal.Destruct.{0} => do
+      let writer : Typewriter.{0,0} τ Tactic := ⟨default, fun next stx => try evalExact stx; catch _ => next stx⟩
+      let (witness, _) ← runTacticMAsMetaM (Typewriter.print writer) δ.mvars.toArray.toList
+      match Parser.runParserCategory (← getEnv) `tactic witness "«standard»" with
+      | .ok stx => return ⟨← `(tactic|intro _; $(⟨stx⟩))⟩
+      | .error err => throwErrorAt (← delab body) err
+  | _ => throwPostpone
+
+def mkFreshGamma (type : Expr := .app (.const ``Universal [levelZero]) (.const ``Universal.Destruct [levelZero])) : MetaM Expr := by
+  refine Meta.mkFreshExprMVar (mkForall `«τ» .implicit ?_ type)
+  exact .app (.const ``Sodium [levelZero]) (.const ``Universal.Destruct [levelZero])
+
+def runRuleOnce (rule : RuleTac := framerule) (deps : Array MVarId := #[]) : MetaM (Array MVarId) := do
+  have : Ord MVarId := ⟨fun α β => α.name.quickCmp β.name⟩
+  let γ ← mkFreshGamma
+  let τ : Expr := .app (.const ``Sodium [levelZero]) (.const ``Universal.Destruct [levelZero])
+  let stx ← Meta.mkAppOptM ``Sodium.Crypto.Verified #[mkConst ``Syntax.Tactic, none]
+  let fwd : Expr := by
+    refine .forallE `«z» stx ?_ .default
+    refine .forallE `«o» (.const ``Observable [levelZero]) ?_ .default
+    refine .app (.app (.const ``Eq [levelZero]) ?_) ?_
+    refine .app (.const ``Observable.Shape.pull [levelZero]) ?_
+    refine .app (.const ``Observable.Shape.push [levelZero]) ?_
+    repeat exact .bvar default
+  let input := {
+    goal := γ.mvarId!
+    mvars := (UnorderedArraySet.ofArray deps).insert γ.mvarId!
+    indexMatchLocations := default
+    patternSubsts? := default
+    options := {generateScript := true, forwardMaxDepth? := none}
+    hypTypes := (∅ : PHashSet _)
+      |>.insert ⟨τ, pinfHash τ⟩
+      |>.insert ⟨fwd, pinfHash fwd⟩
+      |>.insert ⟨stx, pinfHash stx⟩
+  }
+  let (out, _) ← BaseM.run (rule input)
+  match out.applications[0]? with
+  | some app => app.postState.restore; return app.goals.map (·.mvarId)
+  | _ => throwPostpone
+
+def runRuleForever (rule : RuleTac := framerule) : MetaM Unit := do
+  let mut mvars : Array MVarId := #[]
+  repeat try mvars ← runRuleOnce rule mvars catch
+  | ex@(.internal id ..) =>
+    if id == Meta.isDefEqStuckExceptionId then
+      IO.FS.Stream.writeLspNotification (← IO.getStdout) {
+        method := "$/exception/stuck"
+        param := json% null
+      }
+    unless id == postponeExceptionId do throw ex
+  | .error stx msg =>
+    IO.FS.Stream.writeLspNotification (← IO.getStdout) {
+      method := "$/exception"
+      param := json% [$(toString stx.prettyPrint), $(← msg.toString)]
+    }
