Sodium/Ethos/Possibly.lean
@@ -1,0 +1,19 @@
+import Sodium.Ethos.Weight
+import Sodium.Crypto.Monad
+
+open Lean Sodium Crypto
+
+namespace Ethos
+
+/--
+Defined for pedagogical completeness.
+-/
+def Prob {σ} {τ : Sodium σ} (x : Weight) := {x : SecretVector τ (x.quantize .global) // x.isZero}
+
+notation "Δ% " x => @Prob _ _ x
+notation "δ% " x => Σ' τ : Sodium (PLift (@default Prop _)), @Prob (PLift (@default Prop _)) τ x
+
+#check Δ% Δ(1 | 3)
+#check δ% Δ(0 | 1)
+
+end Ethos
