Sodium/Lean/DiscrTree.lean
@@ -1,4 +1,3 @@
-import Aesop
 import Sodium.Lean.Syntax
 
 namespace Lean.Meta
@@ -17,9 +16,7 @@ instance Literal.encodable : Encodable Literal := Encodable.ofEquiv (Nat ⊕ Str
     | .inr s => .strVal s
 }
 
-namespace DiscrTree
-
-namespace Key
+namespace DiscrTree.Key
 
 def Shape :=
   Fin 3
@@ -30,7 +27,7 @@ def Shape :=
 
 instance Shape.encodable : Encodable Shape := by unfold Shape; infer_instance
 
-def toShape : Key → Shape
+def Shape.push : Key → Shape
   | star => .inl 0
   | arrow => .inl 1
   | other => .inl 2
@@ -39,7 +36,7 @@ def toShape : Key → Shape
   | const x n => .inr (.inr (.inr (.inl ⟨x, n⟩)))
   | proj x n₁ n₂ => .inr (.inr (.inr (.inr ⟨x, n₁, n₂⟩)))
 
-def ofShape : Shape → Key
+def Shape.pull : Shape → Key
   | .inl 0 => star
   | .inl 1 => arrow
   | .inl 2 => other
@@ -50,55 +47,10 @@ def ofShape : Shape → Key
 
 instance encodable : Encodable Key :=
   Encodable.ofEquiv _ {
-    push := toShape
-    pull := ofShape
+    push := Shape.push
+    pull := Shape.pull
   }
 
-end Key
-
-namespace Trie
-
-variable {α} [Encodable α]
-
-def Shape := Json × Array Json
-
-instance : Encodable Shape := by unfold Shape; infer_instance
-
-def Shape.arity : Shape → Nat
-  | ⟨_, ks⟩ => ks.size
-
-def Shape.push : Trie α → WType fun i : Shape => Fin i.arity
-  | .node ns nk => by
-    refine ⟨⟨encode ns, nk.map fun ⟨n, _⟩ => encode n⟩, fun i => ?_⟩
-    simp [arity] at i
-    cases h : nk.size with
-    | zero =>
-      rw [h] at i
-      exact Fin.elim0 i
-    | succ n =>
-      let k := nk[i].2
-      exact Shape.push k
-decreasing_by
-  sorry
-
-def Shape.pull : WType (fun i : Shape => Fin i.arity) → Option (Trie α)
-  | ⟨⟨x, #[]⟩, _⟩ => do
-    let ns ← decode? (α := Array α) x
-    return .node ns #[]
-  | ⟨⟨x, ks⟩, f⟩ => do
-    let ns ← decode? (α := Array α) x
-    let nk ← Array.mapM id <| Array.ofFn (n := ks.size) id |>.map fun i => do
-      let k ← decode? (α := Key) (ks[i]'i.isLt)
-      let n ← Shape.pull (f i)
-      return ⟨k, n⟩
-    return .node ns nk
-
-instance encodable : Encodable (Trie α) :=
-  Encodable.ofLeftInj Shape.push Shape.pull fun x => by
-    sorry
-
-end Trie
-
-end DiscrTree
+end DiscrTree.Key
 
 end Lean.Meta
